finished lambda beta example

PROP_untyped/ex_ulcbeta.v
@@ -1,13 +1,12 @@
 Require Export CatSem.PROP_untyped.prop_arities_initial.
 
+Require Import Coq.Program.Equality.
+
 Set Implicit Arguments.
 Unset Strict Implicit.
 Unset Automatic Introduction.
 Unset Transparent Obligations.
 
-Check sub.
-
-Print Signature.
 
 Inductive Lambda_index := ABS | APP.
 
@@ -19,16 +18,18 @@ Definition Lambda : Signature := {|
                   end
 |}.
 
-Print half_eq_classic.
-Check subst_half.
-Definition Lambda_subst := subst_half Lambda.
+(*Definition Lambda_subst := subst_half_eq Lambda.
 Check Lambda_subst.
+*)
 
 Section App_Abs_half_eq.
 
+
+Section for_a_representation.
+
 Variable R : REP Lambda.
 
-Definition blubb1  :
+Definition beta_carrier :
 (forall c : TYPE, (S_Mod_classic_ob [[1; 0]] R) c ---> (S_Mod_classic_ob [[0]] R) c) .
 simpl.
 intros.
@@ -41,16 +42,12 @@ constructor.
 simpl.
 destruct R as [Rr Repr].
 simpl in *.
-set (HH := Repr APP).
-simpl in HH.
-destruct HH.
-simpl in *.
-apply rmodule_hom.
+apply (Repr APP).
+simpl.
 simpl in *.
 constructor.
 simpl.
-set (HH1 := Repr ABS).
-apply HH1.
+apply (Repr ABS).
 simpl.
 constructor.
 simpl.
@@ -63,6 +60,88 @@ constructor.
 constructor.
 Defined.
 
+Program Instance beta_struct  : RModule_Hom_struct 
+  (M:=S_Mod_classic_ob [[1;0]] R) (N:=S_Mod_classic_ob [[0]] R) beta_carrier.
+Next Obligation.
+Proof.
+  dependent destruction x.
+  simpl.
+  dependent destruction x.
+  simpl in *.
+  apply CONSTR_eq; auto.
+  destruct R.
+  simpl in *.
+  rerew (rmhom_rmkl (repr APP)).
+  apply f_equal.
+  simpl in *.
+  apply CONSTR_eq; auto.
+  clear x.
+  clear p0.
+  rerew (rmhom_rmkl (repr ABS)).
+Qed.
+
+Definition beta_module_mor := Build_RModule_Hom beta_struct.
+
+End for_a_representation.
+
+Program Instance beta_half_s : half_equation_struct 
+      (U:=Build_S_Module (S_Mod_classic Lambda [[1 ; 0]])) 
+      (V:=S_Mod_classic Lambda [[0]]) 
+      beta_module_mor.
+Next Obligation.
+Proof.
+  
+  dependent destruction x.
+  dependent destruction x.
+  dependent destruction x.
+  
+  simpl.
+  apply CONSTR_eq; auto.
+  destruct S; simpl.
+  destruct R; simpl.
+  assert (H:=@repr_hom_s _ _ _ _ f).
+  simpl in *.
+  assert (Habs := H ABS).
+  simpl in *.
+  unfold commute in Habs; simpl in *.
+  assert (Happ := H APP).
+  simpl in *.
+  unfold commute in Happ; simpl in *.
+  rewrite <- Happ.
+  apply f_equal.
+  simpl in *.
+  apply CONSTR_eq; auto.
+  rewrite <- Habs.
+  auto.
+Qed.
+  
+
+Definition beta_half_eq := Build_half_equation beta_half_s.
+
 
 End App_Abs_half_eq.
+
+
+Definition beta_rule : eq_classic Lambda := {|
+   eq1 := beta_half_eq ;
+   eq2 := subst_half_eq Lambda |}.
+
+Print beta_rule.
+
+
+
+
+
+
+
+
+
+
+
+
+
+
+
+
+
 
